feat: implement beacon styles

DynamoDbEncryption/runtimes/java/src/main/smithy-generated/software/amazon/cryptography/dbencryptionsdk/dynamodb/model/TwinnedSet.java
@@ -1,0 +1,76 @@
+// Copyright Amazon.com Inc. or its affiliates. All Rights Reserved.
+// SPDX-License-Identifier: Apache-2.0
+// Do not modify this file. This file is machine generated, and any changes to it will be overwritten.
+package software.amazon.cryptography.dbencryptionsdk.dynamodb.model;
+
+import java.util.Objects;
+
+/**
+ * Both Twinned and AsSet.
+ */
+public class TwinnedSet {
+  /**
+   * Calculate beacon values as for this beacon.
+   */
+  private final String other;
+
+  protected TwinnedSet(BuilderImpl builder) {
+    this.other = builder.other();
+  }
+
+  /**
+   * @return Calculate beacon values as for this beacon.
+   */
+  public String other() {
+    return this.other;
+  }
+
+  public Builder toBuilder() {
+    return new BuilderImpl(this);
+  }
+
+  public static Builder builder() {
+    return new BuilderImpl();
+  }
+
+  public interface Builder {
+    /**
+     * @param other Calculate beacon values as for this beacon.
+     */
+    Builder other(String other);
+
+    /**
+     * @return Calculate beacon values as for this beacon.
+     */
+    String other();
+
+    TwinnedSet build();
+  }
+
+  static class BuilderImpl implements Builder {
+    protected String other;
+
+    protected BuilderImpl() {
+    }
+
+    protected BuilderImpl(TwinnedSet model) {
+      this.other = model.other();
+    }
+
+    public Builder other(String other) {
+      this.other = other;
+      return this;
+    }
+
+    public String other() {
+      return this.other;
+    }
+
+    public TwinnedSet build() {
+      if (Objects.isNull(this.other()))  {
+        throw new IllegalArgumentException("Missing value for required field `other`");
+      }
+      return new TwinnedSet(this);
+    }
+  }
+}
